

# CENG 223

## Discrete Computational Structures

Fall '2020-2021

### Homework 3

Student Name and Surname: Mustafa Ilbey Deniz

Student Number: 244831

---

#### Question 1

By Fermat's Little Theorem,

$$2^{22} = 4^{11} \equiv 4 \pmod{11}$$

$$4^{44} = (4^4)^{11} \equiv 4^4 \equiv 256 \equiv 3 \pmod{11}$$

$$6^{66} = (6^6)^{11} \equiv 6^6 \equiv 36 * 36 * 36 \equiv 3 * 3 * 3 \equiv 5 \pmod{11}$$

$$8^{88} = (8^8)^{11} \equiv 8^8 \equiv 2^{24} \equiv 4^{11} * 4 \equiv 4 * 4 \equiv 5 \pmod{11}$$

$$10^{110} = (10^{10})^{11} \equiv 10^{10} \equiv 1 \pmod{11}$$

Therefore,

$$4 + 3 + 5 + 5 + 1 \equiv 7 \pmod{11}$$

#### Question 2

$$7n + 4 = (5n + 3) * 1 + 2n + 1$$

$$5n + 3 = (2n + 1) * 2 + n + 1$$

$$2n + 1 = (n + 1) * 1 + n$$

$$n + 1 = (n) * 1 + 1$$

$$n = (1) * n + 0$$

Therefore,  $\gcd(7n + 4, 5n + 3) = 1$ .

## Question 3

Given that  $m^2 = n^2 + kx$ ,

$$m^2 - n^2 = kx$$

$$(m + n)(m - n) = kx$$

$$x \mid (m + n)(m - n)$$

Suppose  $p \mid (m - n)$  is false, which results in  $\gcd(m-n, p) = 1$  since  $p$  is prime. By Euclid's Lemma, which states if  $a \mid bc$  and  $\gcd(a, b) = 1$ , then  $a \mid c$  must be true where  $a, b, c$  are integers,

$$x \mid (m + n)$$

must be true. The case where  $p \mid (m + n)$  is false is similar. Therefore  $x \mid (m + n)$  or  $x \mid (m - n)$  must be true.

## Question 4

(Base case) For  $n=1$ ,  $\frac{n(3n-1)}{2} = 1$  is true. For some  $n=k$ , say

$$1 + 4 + 7 \dots 3k - 2 = \frac{k(3k - 1)}{2}$$

If it is also true for  $n=k+1$ , this will prove our claim.

$$\frac{k(3k - 1)}{2} + 3k + 1 \stackrel{?}{=} \frac{(k + 1)(3k + 2)}{2}$$

$$k(3k - 1) + 6k + 2 \stackrel{?}{=} (k + 1)(3k + 2)$$

$$3k^2 - k + 6k + 2 = 3k^2 + 2k + 3k + 2$$

Therefore, our claim is true for  $n=k+1$  which makes our claim true for all  $n \geq 1$ .